src/Constants.fst
@@ -1,0 +1,35 @@
+module Constants
+
+module U32 = FStar.UInt32
+
+open FStar.Mul
+
+// LATER: code could be improved so that this value is not hardcoded anymore
+inline_for_extraction
+let page_size: U32.t = 4096ul
+
+noextract
+let min_sc = 64
+noextract
+let max_sc = U32.v page_size
+
+// TODO: this could be improved
+// currently does not support size classes
+// such that:
+// - sc < 64, thus nb_slot sc > 64
+// and
+// - (nb_slots sc) % 64 <> 0
+// this allows to only have a particular mechanism
+// for the first u64 of the bitmap
+// note: this mechanism does not rely on any loop!
+let sc = x:U32.t{
+  (
+    U32.eq x 16ul \/
+    U32.eq x 32ul \/
+    (min_sc <= U32.v x /\ U32.v x <= max_sc)
+  ) /\
+  // https://www.intel.com/content/dam/develop/external/us/en/documents/mpx-linux64-abi.pdf
+  // allocated arrays should have alignment of at least 16 bytes,
+  // allowing use of SSE instructions
+  (U32.v x % 16 == 0)
+}
