src/SizeClass.fst
@@ -17,6 +17,7 @@ open Steel.Effect.Atomic
 open Steel.Effect
 open Steel.Reference
 
+open Constants
 open Config
 open Utils2
 
